theories/iris/diaframe/symb_exec/defs.v
@@ -1,0 +1,2 @@
+From diaframe Require Export
+  symb_exec.defs.
