theories/iris/program_logic/adequacy.v
@@ -1,0 +1,174 @@
+From zebre Require Import
+  prelude.
+From zebre.iris.bi Require Import
+  big_op.
+From zebre.iris Require Import
+  diaframe.
+From zebre.iris.program_logic Require Export
+  wp.
+From zebre Require Import
+  options.
+
+Section iris_G.
+  Context `{iris_G : !IrisG Λ Σ}.
+
+  Implicit Types e : expr Λ.
+  Implicit Types es : list (expr Λ).
+  Implicit Types Φ : val Λ → iProp Σ.
+  Implicit Types Φs : list (val Λ → iProp Σ).
+
+  Definition wps es Φs : iProp Σ :=
+    [∗ list] e; Φ ∈ es; Φs,
+      WP e @ ⊤ {{ Φ }}.
+
+  #[local] Lemma wp_step e1 σ1 e2 σ2 κ κs es ϕ Φ :
+    prim_step e1 σ1 κ e2 σ2 es ϕ →
+    ϕ →
+    state_interp σ1 (κ ++ κs) -∗
+    £ 1 -∗
+    WP e1 @ ⊤ {{ Φ }} -∗
+      |={⊤}[∅]▷=>
+      state_interp σ2 κs ∗
+      WP e2 @ ⊤ {{ Φ }} ∗
+      wps es (replicate (length es) fork_post).
+  Proof.
+    iIntros "%Hstep %Hϕ Hσ H£ H".
+    rewrite {1}wp_unfold /wp_pre (val_stuck e1 σ1 κ e2 σ2 es ϕ) //.
+    iMod ("H" with "Hσ") as "(_ & H)".
+    iMod ("H" with "[//] [//] H£") as "H".
+    iModIntro. iSteps. rewrite /wps big_sepL2_replicate_r //.
+  Qed.
+
+  #[local] Lemma wps_step es1 σ1 es2 σ2 κ κs ϕ Φs :
+    step (es1, σ1) κ (es2, σ2) ϕ →
+    ϕ →
+    state_interp σ1 (κ ++ κs) -∗
+    £ 1 -∗
+    wps es1 Φs -∗
+      |={⊤}[∅]▷=>
+      ∃ n_forked,
+      state_interp σ2 κs ∗
+      wps es2 (Φs ++ replicate n_forked fork_post).
+  Proof.
+    iIntros "%Hstep %Hϕ Hσ H£ H".
+    destruct Hstep as [e1 σ1' e2 σ2' es es1' es2' Hstep]; simplify_eq/=.
+    iDestruct (big_sepL2_app_inv_l with "H") as (Φs1 Φs2 ->) "(Hes1' & H)".
+    iDestruct (big_sepL2_cons_inv_l with "H") as (Φ Φs3 ->) "(He1 & Hes2')".
+    iMod (wp_step with "Hσ H£ He1") as "H"; [done.. |].
+    iExists _. rewrite -(assoc (++)) -app_comm_cons. iFrame. iSteps.
+  Qed.
+
+  #[local] Lemma wps_steps n es1 σ1 es2 σ2 κs1 κs2 ϕs Φs :
+    nsteps n (es1, σ1) κs1 (es2, σ2) ϕs →
+    Forall id ϕs →
+    state_interp σ1 (κs1 ++ κs2) -∗
+    £ n -∗
+    wps es1 Φs -∗
+      |={⊤,∅}=> |={∅}▷=>^n |={∅,⊤}=>
+      ∃ n_forked,
+      state_interp σ2 κs2 ∗
+      wps es2 (Φs ++ replicate n_forked fork_post).
+  Proof.
+    iInduction n as [| n] "IH" forall (es1 σ1 κs1 κs2 ϕs Φs) => /=.
+    all: iIntros "%Hsteps %Hϕs Hσ H£s H".
+    - invert Hsteps.
+      iExists 0. rewrite right_id. iSteps.
+    - invert Hsteps as [| ? ? (es1' & σ1') ? κ κs1' ϕ ϕs' Hstep Hsteps'].
+      apply Forall_cons in Hϕs as (Hϕ & Hϕs').
+      rewrite -(assoc (++)).
+      iDestruct "H£s" as "(H£ & H£s)".
+      iMod (wps_step with "Hσ H£ H") as "H"; [done.. |].
+      do 3 iModIntro.
+      iApply (fupd_trans _ ⊤).
+      iMod "H" as "(%n_forked & Hσ & H)".
+      iModIntro.
+      iMod ("IH" with "[//] [//] Hσ H£s H") as "H"; [done.. |].
+      iModIntro.
+      iApply (step_fupdN_wand with "H"). iIntros ">H".
+      iDestruct "H" as "(%n_forked' & Hσ & H)".
+      rewrite -(assoc app) -replicate_add. iSteps.
+  Qed.
+
+  #[local] Lemma wp_not_stuck e σ κs Φ :
+    state_interp σ κs -∗
+    WP e {{ Φ }} -∗
+      |={⊤, ∅}=>
+      ⌜not_stuck e σ⌝.
+  Proof.
+    iIntros "Hσ H".
+    rewrite wp_unfold /wp_pre /not_stuck.
+    destruct (to_val e) as [v |] eqn:He.
+    - iMod (fupd_mask_subseteq ∅); first done.
+      iSteps.
+    - iSpecialize ("H" $! σ [] κs with "Hσ").
+      iMod "H" as "(%Hreducible & _)".
+      iSteps.
+  Qed.
+
+  #[local] Lemma wps_progress n es1 σ1 e2 es2 σ2 κs1 κs2 ϕs Φs :
+    nsteps n (es1, σ1) κs1 (es2, σ2) ϕs →
+    Forall id ϕs →
+    e2 ∈ es2 →
+    state_interp σ1 (κs1 ++ κs2) -∗
+    £ n -∗
+    wps es1 Φs -∗
+      |={⊤, ∅}=> |={∅}▷=>^n |={∅}=>
+      ⌜not_stuck e2 σ2⌝.
+  Proof.
+    iIntros (Hsteps Hϕs (i & Hes2_lookup)%elem_of_list_lookup) "Hσ H£s He".
+    iMod (wps_steps with "Hσ H£s He") as "H"; [done.. |].
+    iModIntro.
+    iApply (step_fupdN_wand with "H").
+    iMod 1 as "(%n_forked & Hσ & H)".
+    iDestruct (big_sepL2_lookup_Some_l with "H") as %(Φ & Hposts_lookup); first done.
+    iDestruct (big_sepL2_lookup with "H") as "H"; [done.. |].
+    iApply (wp_not_stuck with "Hσ H").
+  Qed.
+End iris_G.
+
+Lemma wp_progress Λ Σ `{inv_Gpre : !invGpreS Σ} n es1 σ1 e2 es2 σ2 κs ϕs :
+  ( ∀ `{inv_G : !invGS Σ},
+    ⊢ |={⊤}=>
+      ∃ state_interp fork_post Φs,
+      let iris_G : IrisG Λ Σ := Build_IrisG state_interp fork_post in
+      state_interp σ1 κs ∗
+      wps es1 Φs
+  ) →
+  nsteps n (es1, σ1) κs (es2, σ2) ϕs →
+  Forall id ϕs →
+  e2 ∈ es2 →
+  not_stuck e2 σ2.
+Proof.
+  intros H Hsteps Hϕs He2.
+  eapply uPred.pure_soundness, (step_fupdN_soundness_lc _ n n).
+  iIntros "%Hinv_G H£s".
+  iMod H as "(%state_interp & %fork_post & %Φs & Hσ & H)".
+  iMod (wps_progress (iris_G := Build_IrisG state_interp fork_post) with "[Hσ] H£s H") as "H"; [done.. | |].
+  { erewrite app_nil_r. done. }
+  destruct n.
+  - iMod "H". iSteps.
+  - iApply step_fupdN_S_fupd. iSteps.
+Qed.
+
+Definition adequate {Λ} (e : expr Λ) σ :=
+  ∀ n κs e' es σ' ϕs,
+  nsteps n ([e], σ) κs (es, σ') ϕs →
+  Forall id ϕs →
+  e' ∈ es →
+  not_stuck e' σ'.
+
+Lemma wp_adequacy Λ Σ `{inv_Gpre : !invGpreS Σ} e σ :
+  ( ∀ `{inv_G : !invGS Σ} κs,
+    ⊢ |={⊤}=>
+      ∃ state_interp fork_post Φ,
+      let iris_G : IrisG Λ Σ := Build_IrisG state_interp fork_post in
+      state_interp σ κs ∗
+      WP e {{ Φ }}
+  ) →
+  adequate e σ.
+Proof.
+  intros H n κs e' es σ' ϕs.
+  apply: wp_progress => inv_G.
+  iMod H as "(%state_interp & %fork_post & %Φ & Hσ & H)".
+  iExists state_interp, fork_post, [Φ]. rewrite /wps /=. iSteps.
+Qed.
