theories/iris/program_logic/atomic.v
@@ -4,13 +4,13 @@ From iris.bi Require Export
   lib.atomic.
 From iris.base_logic Require Import
   lib.invariants.
-From iris.program_logic Require Export
-  weakestpre.
 
 From zebre Require Import
   prelude.
 From zebre.iris Require Import
   diaframe.
+From zebre.iris.program_logic Require Export
+  wp.
 From zebre Require Import
   options.
 
@@ -143,7 +143,7 @@ Section atomic_update.
 End atomic_update.
 
 Section atomic_wp.
-  Context `{iris_GS : !irisGS Λ Σ} {TA TB : tele}.
+  Context `{iris_GS : !IrisG Λ Σ} {TA TB : tele}.
 
   Implicit Types α : TA → iProp Σ.
   Implicit Types β Ψ : TA → TB → iProp Σ.
@@ -239,27 +239,6 @@ Section atomic_wp.
     iIntros "H %Φ HΦ".
     iDestruct (atomic_update_mask_weaken _ (⊤ ∖ E1) with "HΦ") as "HΦ"; first solve_ndisj.
     iSteps.
-  Qed.
-
-  Lemma atomic_wp_seq e E α β Ψ f :
-    atomic_wp e E α β Ψ f ⊢
-    ∀ Φ, ∀.. x, α x -∗ (∀.. y, β x y -∗ Ψ x y -∗ Φ (f x y)) -∗ WP e {{ Φ }}.
-  Proof.
-    iIntros "H %Φ %x Hα HΦ".
-    iApply (wp_frame_wand with "HΦ").
-    iApply "H".
-    iAuIntro. iAaccIntro with "Hα"; first auto. iIntros "%y Hβ !>". rewrite !tele_app_bind. iIntros "HΨ HΦ".
-    iApply ("HΦ" with "Hβ HΨ").
-  Qed.
-  Lemma atomic_wp_seq_step e E α β Ψ f :
-    to_val e = None →
-    atomic_wp e E α β Ψ f ⊢
-    ∀ Φ, ∀.. x, α x -∗ ▷ (∀.. y, β x y -∗ Ψ x y -∗ Φ (f x y)) -∗ WP e {{ Φ }}.
-  Proof.
-    iIntros "% H %Φ %x Hα HΦ".
-    iApply (wp_step_fupd _ _ _ _ (∀.. y, β x y -∗ Ψ x y -∗ Φ (f x y)) with "[$HΦ //]"); [rewrite TCEq_eq // | done |].
-    iApply (atomic_wp_seq with "H Hα"). iIntros "%y Hβ HΨ HΦ".
-    iApply ("HΦ" with "Hβ HΨ").
   Qed.
 End atomic_wp.
 
@@ -393,7 +372,7 @@ Notation "'AWP' '<<' α '>>' e '<<' β | 'RET' v ; Q '>>'" := (
 ) : bi_scope.
 
 Section atomic_triple.
-  Context `{!irisGS Λ Σ} {TA TB : tele}.
+  Context `{iris_G : !IrisG Λ Σ} {TA TB : tele}.
 
   Implicit Types P : iProp Σ.
   Implicit Types α : TA → iProp Σ.
@@ -496,27 +475,6 @@ Section atomic_triple.
     iIntros "#H !> %Φ HP HΦ".
     iDestruct (atomic_update_mask_weaken _ (⊤ ∖ E1) with "HΦ") as "HΦ"; first solve_ndisj.
     iSteps.
-  Qed.
-
-  Lemma atomic_triple_seq e E P α β Ψ f :
-    atomic_triple e E P α β Ψ f ⊢
-    □ ∀ Φ, P -∗ ∀.. x, α x -∗ (∀.. y, β x y -∗ Ψ x y -∗ Φ (f x y)) -∗ WP e {{ Φ }}.
-  Proof.
-    iIntros "#H !> %Φ HP %x Hα HΦ".
-    iApply (wp_frame_wand with "HΦ").
-    iApply ("H" with "HP").
-    iAuIntro. iAaccIntro with "Hα"; first auto. iIntros "%y Hβ !>". rewrite !tele_app_bind. iIntros "HΨ HΦ".
-    iApply ("HΦ" with "Hβ HΨ").
-  Qed.
-  Lemma atomic_triple_seq_step e E P α β Ψ f :
-    to_val e = None →
-    atomic_triple e E P α β Ψ f ⊢
-    □ ∀ Φ, P -∗ ∀.. x, α x -∗ ▷ (∀.. y, β x y -∗ Ψ x y -∗ Φ (f x y)) -∗ WP e {{ Φ }}.
-  Proof.
-    iIntros "% #H !> %Φ HP %x Hα HΦ".
-    iApply (wp_step_fupd _ _ _ _ (∀.. y, β x y -∗ Ψ x y -∗ Φ (f x y)) with "[$HΦ //]"); [rewrite TCEq_eq // | done |].
-    iApply (atomic_triple_seq with "H HP Hα"). iIntros "%y Hβ HΨ HΦ".
-    iApply ("HΦ" with "Hβ HΨ").
   Qed.
 End atomic_triple.
 
