theories/iris/program_logic/ectx_language.v
@@ -1,0 +1,400 @@
+From zebre Require Import
+  prelude.
+From zebre.iris.program_logic Require Import
+  language.
+From zebre Require Import
+  options.
+
+Section ectx_language_mixin.
+  Context {expr val ectx state observation : Type}.
+  Context (of_val : val → expr).
+  Context (to_val : expr → option val).
+  Context (empty_ectx : ectx).
+  Context (comp_ectx : ectx → ectx → ectx).
+  Context (fill : ectx → expr → expr).
+  Context (base_step : expr → state → list observation → expr → state → list expr → Prop → Prop).
+
+  Record EctxLanguageMixin := {
+    mixin_to_of_val v :
+      to_val (of_val v) = Some v ;
+    mixin_of_to_val e v :
+      to_val e = Some v →
+      of_val v = e ;
+    mixin_val_base_stuck e1 σ1 κ e2 σ2 es ϕ :
+      base_step e1 σ1 κ e2 σ2 es ϕ →
+      to_val e1 = None ;
+
+    mixin_fill_empty e :
+      fill empty_ectx e = e ;
+    mixin_fill_comp K1 K2 e :
+      fill K1 (fill K2 e) = fill (comp_ectx K1 K2) e ;
+    mixin_fill_inj K :
+      Inj (=) (=) (fill K) ;
+    mixin_fill_val K e :
+      is_Some (to_val (fill K e)) →
+      is_Some (to_val e) ;
+
+    mixin_step_by_val K' K_redex e1' e1_redex σ1 κ e2 σ2 es ϕ :
+      fill K' e1' = fill K_redex e1_redex →
+      to_val e1' = None →
+      base_step e1_redex σ1 κ e2 σ2 es ϕ →
+        ∃ K'',
+        K_redex = comp_ectx K' K'' ;
+
+    mixin_base_ctx_step_val K e σ1 κ e2 σ2 es ϕ :
+      base_step (fill K e) σ1 κ e2 σ2 es ϕ →
+        is_Some (to_val e) ∨
+        K = empty_ectx ;
+  }.
+End ectx_language_mixin.
+
+Structure ectx_language := {
+  expr : Type ;
+  val : Type ;
+  ectx : Type ;
+  state : Type ;
+  observation : Type ;
+
+  of_val : val → expr ;
+  to_val : expr → option val ;
+  empty_ectx : ectx ;
+  comp_ectx : ectx → ectx → ectx ;
+  fill : ectx → expr → expr ;
+  base_step : expr → state → list observation → expr → state → list expr → Prop → Prop ;
+
+  ectx_language_mixin : EctxLanguageMixin of_val to_val empty_ectx comp_ectx fill base_step ;
+}.
+
+Bind Scope expr_scope with expr.
+Bind Scope val_scope with val.
+
+#[global] Arguments Build_ectx_language {_ _ _ _ _ _ _ _ _ _ _} _ : assert.
+#[global] Arguments of_val {_} _ : assert.
+#[global] Arguments to_val {_} _ : assert.
+#[global] Arguments empty_ectx {_} : assert.
+#[global] Arguments comp_ectx {_} _ _ : assert.
+#[global] Arguments fill {_} _ _ : assert.
+#[global] Arguments base_step {_} _ _ _ _ _ _ _ : assert.
+
+Section ectx_language.
+  Context {Λ : ectx_language}.
+
+  Implicit Types e : expr Λ.
+  Implicit Types v : val Λ.
+  Implicit Types σ : state Λ.
+  Implicit Types K : ectx Λ.
+  Implicit Types κ : list (observation Λ).
+
+  Lemma val_base_stuck e1 σ1 κ e2 σ2 es ϕ :
+    base_step e1 σ1 κ e2 σ2 es ϕ →
+    to_val e1 = None.
+  Proof.
+    apply ectx_language_mixin.
+  Qed.
+  Lemma fill_empty e :
+    fill empty_ectx e = e.
+  Proof.
+    apply ectx_language_mixin.
+  Qed.
+  Lemma fill_comp K1 K2 e :
+    fill K1 (fill K2 e) = fill (comp_ectx K1 K2) e.
+  Proof.
+    apply ectx_language_mixin.
+  Qed.
+  #[global] Instance fill_inj K :
+    Inj (=) (=) (fill K).
+  Proof.
+    apply ectx_language_mixin.
+  Qed.
+  Lemma fill_val K e :
+    is_Some (to_val (fill K e)) →
+    is_Some (to_val e).
+  Proof.
+    apply ectx_language_mixin.
+  Qed.
+  Lemma step_by_val K' K_redex e1' e1_redex σ1 κ e2 σ2 es ϕ :
+    fill K' e1' = fill K_redex e1_redex →
+    to_val e1' = None →
+    base_step e1_redex σ1 κ e2 σ2 es ϕ →
+      ∃ K'',
+      K_redex = comp_ectx K' K''.
+  Proof.
+    apply ectx_language_mixin.
+  Qed.
+  Lemma base_ctx_step_val K e σ1 κ e2 σ2 es ϕ :
+    base_step (fill K e) σ1 κ e2 σ2 es ϕ →
+      is_Some (to_val e) ∨
+      K = empty_ectx.
+  Proof.
+    apply ectx_language_mixin.
+  Qed.
+
+  Definition base_reducible e σ :=
+    ∃ κ e' σ' es ϕ,
+    base_step e σ κ e' σ' es ϕ.
+  Definition base_reducible_no_obs e σ :=
+    ∃ e' σ' es ϕ,
+    base_step e σ [] e' σ' es ϕ.
+  Definition base_irreducible e σ :=
+    ∀ κ e' σ' es ϕ,
+    ¬ base_step e σ κ e' σ' es ϕ.
+  Definition base_stuck e σ :=
+    to_val e = None ∧
+    base_irreducible e σ.
+
+  Definition sub_redexes_are_values e :=
+    ∀ K e', e = fill K e' →
+    to_val e' = None →
+    K = empty_ectx.
+
+  Inductive prim_step e1 σ1 κ e2 σ2 es ϕ : Prop :=
+    | Ectx_step K e1' e2' :
+        e1 = fill K e1' →
+        e2 = fill K e2' →
+        base_step e1' σ1 κ e2' σ2 es ϕ →
+        prim_step e1 σ1 κ e2 σ2 es ϕ.
+
+  Lemma Ectx_step' K e1 σ1 κ e2 σ2 es ϕ :
+    base_step e1 σ1 κ e2 σ2 es ϕ →
+    prim_step (fill K e1) σ1 κ (fill K e2) σ2 es ϕ.
+  Proof.
+    econstructor; eauto.
+  Qed.
+
+  Definition ectx_lang_mixin :
+    LanguageMixin of_val to_val prim_step.
+  Proof.
+    split.
+    - apply ectx_language_mixin.
+    - apply ectx_language_mixin.
+    - intros ? ? ? ? ? ? ? [? ? ? -> -> ?%val_base_stuck].
+      apply eq_None_not_Some. intros ?%fill_val%eq_None_not_Some; done.
+  Qed.
+
+  Canonical ectx_lang :=
+    Build_language ectx_lang_mixin.
+
+  Definition base_atomic e :=
+    ∀ σ κ e' σ' es ϕ,
+    base_step e σ κ e' σ' es ϕ →
+    is_Some (to_val e').
+
+  Lemma fill_not_val K e :
+    to_val e = None →
+    to_val (fill K e) = None.
+  Proof.
+    rewrite !eq_None_not_Some. eauto using fill_val.
+  Qed.
+
+  Lemma base_reducible_no_obs_reducible e σ :
+    base_reducible_no_obs e σ →
+    base_reducible e σ.
+  Proof.
+    intros (? & ? & ? & ?). eexists. eauto.
+  Qed.
+  Lemma not_base_reducible e σ :
+    ¬ base_reducible e σ ↔
+    base_irreducible e σ.
+  Proof.
+    unfold base_reducible, base_irreducible. naive_solver.
+  Qed.
+
+  Lemma base_redex_unique K K' e e' σ :
+    fill K e = fill K' e' →
+    base_reducible e σ →
+    base_reducible e' σ →
+      K = comp_ectx K' empty_ectx ∧
+      e = e'.
+  Proof.
+    intros Heq (κ & e2 & σ2 & es & ϕ & Hred) (κ' & e2' & σ2' & es' & ϕ' & Hred').
+    edestruct (step_by_val K' K e' e) as [K'' HK]; [eauto using val_base_stuck.. |].
+    subst K. move: Heq. rewrite -fill_comp. intros <-%(inj (fill _)).
+    destruct (base_ctx_step_val _ _ _ _ _ _ _ _ Hred') as [[]%not_eq_None_Some | HK''].
+    { eapply val_base_stuck. done. }
+    subst K''. rewrite fill_empty //.
+  Qed.
+
+  Lemma base_prim_step e1 σ1 κ e2 σ2 es ϕ :
+    base_step e1 σ1 κ e2 σ2 es ϕ →
+    prim_step e1 σ1 κ e2 σ2 es ϕ.
+  Proof.
+    apply Ectx_step with empty_ectx; rewrite ?fill_empty //.
+  Qed.
+
+  Lemma base_step_not_stuck e σ κ e' σ' es ϕ :
+    base_step e σ κ e' σ' es ϕ →
+    not_stuck e σ.
+  Proof.
+    rewrite /not_stuck /reducible /=. eauto 10 using base_prim_step.
+  Qed.
+
+  Lemma fill_prim_step K e1 σ1 κ e2 σ2 es ϕ :
+    prim_step e1 σ1 κ e2 σ2 es ϕ →
+    prim_step (fill K e1) σ1 κ (fill K e2) σ2 es ϕ.
+  Proof.
+    destruct 1 as [K' e1' e2' -> ->].
+    rewrite !fill_comp. econstructor; done.
+  Qed.
+  Lemma fill_reducible K e σ :
+    reducible e σ →
+    reducible (fill K e) σ.
+  Proof.
+    intros (κ & e' & σ' & es & ϕ & ?). exists κ, (fill K e'), σ', es, ϕ.
+    apply fill_prim_step. done.
+  Qed.
+  Lemma fill_reducible_no_obs K e σ :
+    reducible_no_obs e σ →
+    reducible_no_obs (fill K e) σ.
+  Proof.
+    intros (e' & σ' & es & ϕ & ?). exists (fill K e'), σ', es, ϕ.
+    apply fill_prim_step. done.
+  Qed.
+  Lemma base_prim_reducible e σ :
+    base_reducible e σ →
+    reducible e σ.
+  Proof.
+    intros (κ & e' & σ' & es & ϕ & ?). eexists κ, e', σ', es, ϕ.
+    apply base_prim_step. done.
+  Qed.
+  Lemma base_prim_fill_reducible e K σ :
+    base_reducible e σ →
+    reducible (fill K e) σ.
+  Proof.
+    intro. apply fill_reducible, base_prim_reducible. done.
+  Qed.
+  Lemma base_prim_reducible_no_obs e σ :
+    base_reducible_no_obs e σ →
+    reducible_no_obs e σ.
+  Proof.
+    intros (e' & σ' & es & ϕ & ?). eexists e', σ', es, ϕ.
+    apply base_prim_step. done.
+  Qed.
+  Lemma base_prim_irreducible e σ :
+    irreducible e σ →
+    base_irreducible e σ.
+  Proof.
+    rewrite -not_reducible -not_base_reducible. eauto using base_prim_reducible.
+  Qed.
+  Lemma base_prim_fill_reducible_no_obs e K σ :
+    base_reducible_no_obs e σ →
+    reducible_no_obs (fill K e) σ.
+  Proof.
+    intro. apply fill_reducible_no_obs, base_prim_reducible_no_obs. done.
+  Qed.
+
+  Lemma prim_base_reducible e σ :
+    reducible e σ →
+    sub_redexes_are_values e →
+    base_reducible e σ.
+  Proof.
+    intros (κ & e' & σ' & es & ϕ & [K e1' e2' -> -> Hstep]) ?.
+    assert (K = empty_ectx) as -> by eauto 10 using val_base_stuck.
+    rewrite fill_empty /base_reducible. eauto 10.
+  Qed.
+  Lemma prim_base_irreducible e σ :
+    base_irreducible e σ →
+    sub_redexes_are_values e →
+    irreducible e σ.
+  Proof.
+    rewrite -not_reducible -not_base_reducible. eauto using prim_base_reducible.
+  Qed.
+
+  Lemma base_stuck_stuck e σ :
+    base_stuck e σ →
+    sub_redexes_are_values e →
+    stuck e σ.
+  Proof.
+    intros [] ?. split; first done.
+    apply prim_base_irreducible; done.
+  Qed.
+
+  Lemma ectx_language_atomic e :
+    base_atomic e →
+    sub_redexes_are_values e →
+    Atomic e.
+  Proof.
+    intros Hatomic_step Hatomic_fill σ κ e' σ' es ϕ [K e1' e2' -> -> Hstep].
+    assert (K = empty_ectx) as -> by eauto 10 using val_base_stuck.
+    rewrite fill_empty. eapply Hatomic_step. rewrite fill_empty //.
+  Qed.
+
+  Lemma base_reducible_prim_step_ctx K e1 σ1 κ e2 σ2 es ϕ :
+    base_reducible e1 σ1 →
+    prim_step (fill K e1) σ1 κ e2 σ2 es ϕ →
+      ∃ e2',
+      e2 = fill K e2' ∧
+      base_step e1 σ1 κ e2' σ2 es ϕ.
+  Proof.
+    intros (κ' & e2'' & σ2'' & es'' & ϕ'' & HhstepK) [K' e1' e2' HKe1 -> Hstep].
+    edestruct (step_by_val K) as [K'' ?]; eauto using val_base_stuck; simplify_eq/=.
+    rewrite -fill_comp in HKe1; simplify_eq.
+    exists (fill K'' e2'). rewrite fill_comp; split; first done.
+    apply base_ctx_step_val in HhstepK as [[v ?] | ?]; simplify_eq.
+    { apply val_base_stuck in Hstep. simplify_eq. }
+    rewrite !fill_empty //.
+  Qed.
+
+  Lemma base_reducible_prim_step e1 σ1 κ e2 σ2 es ϕ :
+    base_reducible e1 σ1 →
+    prim_step e1 σ1 κ e2 σ2 es ϕ →
+    base_step e1 σ1 κ e2 σ2 es ϕ.
+  Proof.
+    intros.
+    edestruct (base_reducible_prim_step_ctx empty_ectx) as (? & ? & ?);
+      rewrite ?fill_empty; eauto.
+    simplify_eq; rewrite fill_empty //.
+  Qed.
+
+  #[global] Instance ectx_lang_ctx K :
+    LanguageCtx (fill K).
+  Proof.
+    split; simpl.
+    - eauto using fill_not_val.
+    - intros ? ? ? ? ? ? ? [K' e1' e2' Heq1 Heq2 Hstep].
+      exists (comp_ectx K K') e1' e2'; rewrite ?Heq1 ?Heq2 ?fill_comp //.
+    - intros e1 σ1 κ e2 σ2 es ϕ Hnval [K'' e1'' e2'' Heq1 -> Hstep].
+      destruct (step_by_val K K'' e1 e1'' σ1 κ e2'' σ2 es ϕ) as [K' ->]; eauto.
+      rewrite -fill_comp in Heq1; apply (inj (fill _)) in Heq1.
+      exists (fill K' e2''); rewrite -fill_comp; split; auto.
+      econstructor; eauto.
+  Qed.
+
+  Record pure_base_step e1 e2 := {
+    pure_base_step_safe σ1 :
+      base_reducible_no_obs e1 σ1 ;
+    pure_base_step_det σ1 κ e2' σ2 es ϕ :
+      base_step e1 σ1 κ e2' σ2 es ϕ →
+        κ = [] ∧
+        σ2 = σ1 ∧
+        e2' = e2 ∧
+        es = [] ;
+  }.
+
+  Lemma pure_base_step_pure_step e1 e2 :
+    pure_base_step e1 e2 →
+    pure_step e1 e2.
+  Proof.
+    intros [Hp1 Hp2]. split.
+    - intros σ. destruct (Hp1 σ) as (e2' & σ2 & es & ϕ & ?).
+      eexists e2', σ2, es, ϕ. apply base_prim_step. done.
+    - intros σ1 κ e2' σ2 es ϕ ?%base_reducible_prim_step;
+        eauto using base_reducible_no_obs_reducible.
+  Qed.
+
+  Lemma pure_exec_fill K ϕ n e1 e2 :
+    PureExec ϕ n e1 e2 →
+    PureExec ϕ n (fill K e1) (fill K e2).
+  Proof.
+    apply: pure_exec_ctx.
+  Qed.
+End ectx_language.
+
+#[global] Arguments Ectx_step {Λ e1 σ1 κ e2 σ2 es ϕ}.
+
+#[global] Arguments ectx_lang : clear implicits.
+Coercion ectx_lang : ectx_language >-> language.
+
+Definition LanguageOfEctx '(Build_ectx_language mixin) : language :=
+  Eval compute in
+  Build_ectx_language mixin.
+#[global] Arguments LanguageOfEctx : simpl never.
