theories/iris/program_logic/language.v
@@ -1,0 +1,358 @@
+From iris.algebra Require Import
+  ofe.
+
+From zebre Require Import
+  prelude.
+From zebre Require Import
+  options.
+
+Section language_mixin.
+  Context {expr val state observation : Type}.
+  Context (of_val : val → expr).
+  Context (to_val : expr → option val).
+  Context (prim_step : expr → state → list observation → expr → state → list expr → Prop → Prop).
+
+  Record LanguageMixin := {
+    mixin_to_of_val v :
+      to_val (of_val v) = Some v ;
+    mixin_of_to_val e v :
+      to_val e = Some v →
+      of_val v = e ;
+    mixin_val_stuck e σ κ e' σ' es ϕ :
+      prim_step e σ κ e' σ' es ϕ →
+      to_val e = None ;
+  }.
+End language_mixin.
+
+Structure language := {
+  expr : Type ;
+  val : Type ;
+  state : Type ;
+  observation : Type ;
+  of_val : val → expr ;
+  to_val : expr → option val ;
+  prim_step : expr → state → list observation → expr → state → list expr → Prop → Prop ;
+  language_mixin : LanguageMixin of_val to_val prim_step ;
+}.
+#[global] Arguments Build_language {_ _ _ _ _ _ _} _ : assert.
+#[global] Arguments of_val {_} _ : assert.
+#[global] Arguments to_val {_} _ : assert.
+#[global] Arguments prim_step {_} _ _ _ _ _ _ _ : assert.
+
+Implicit Types Λ : language.
+
+Declare Scope expr_scope.
+Delimit Scope expr_scope with E.
+
+Declare Scope val_scope.
+Delimit Scope val_scope with V.
+
+Bind Scope expr_scope with expr.
+Bind Scope val_scope with val.
+
+Canonical state_O Λ :=
+  leibnizO (state Λ).
+Canonical val_O Λ :=
+  leibnizO (val Λ).
+Canonical expr_O Λ :=
+  leibnizO (expr Λ).
+
+Definition config Λ : Type :=
+  list (expr Λ) * state Λ.
+
+Class LanguageCtx {Λ} (K : expr Λ → expr Λ) := {
+  fill_not_val e :
+    to_val e = None →
+    to_val (K e) = None ;
+  fill_step e1 σ1 κ e2 σ2 es ϕ :
+    prim_step e1 σ1 κ e2 σ2 es ϕ →
+    prim_step (K e1) σ1 κ (K e2) σ2 es ϕ ;
+  fill_step_inv e1' σ1 κ e2 σ2 es ϕ :
+    to_val e1' = None →
+    prim_step (K e1') σ1 κ e2 σ2 es ϕ →
+      ∃ e2',
+      e2 = K e2' ∧
+      prim_step e1' σ1 κ e2' σ2 es ϕ ;
+}.
+
+#[global] Instance language_ctx_id Λ :
+  LanguageCtx (@id (expr Λ)).
+Proof.
+  constructor; naive_solver.
+Qed.
+
+Section language.
+  Context {Λ}.
+
+  Implicit Types e : expr Λ.
+  Implicit Types v : val Λ.
+  Implicit Types σ : state Λ.
+  Implicit Types ρ : config Λ.
+  Implicit Types κ : list (observation Λ).
+
+  Lemma to_of_val v :
+    to_val (of_val v) = Some v.
+  Proof.
+    apply language_mixin.
+  Qed.
+  Lemma of_to_val e v :
+    to_val e = Some v →
+    of_val v = e.
+  Proof.
+    apply language_mixin.
+  Qed.
+  Lemma val_stuck e σ κ e' σ' es ϕ :
+    prim_step e σ κ e' σ' es ϕ →
+    to_val e = None.
+  Proof.
+    apply language_mixin.
+  Qed.
+
+  Definition reducible e σ :=
+    ∃ κ e' σ' es ϕ,
+    prim_step e σ κ e' σ' es ϕ.
+  Definition reducible_no_obs e σ :=
+    ∃ e' σ' es ϕ,
+    prim_step e σ [] e' σ' es ϕ.
+  Definition irreducible e σ :=
+    ∀ κ e' σ' es ϕ,
+    ¬ prim_step e σ κ e' σ' es ϕ.
+  Definition stuck e σ :=
+    to_val e = None ∧
+    irreducible e σ.
+  Definition not_stuck e σ :=
+    is_Some (to_val e) ∨
+    reducible e σ.
+
+  Class Atomic e :=
+    atomic σ e' κ σ' es ϕ :
+      prim_step e σ κ e' σ' es ϕ →
+      is_Some (to_val e').
+
+  Inductive step ρ1 κ ρ2 ϕ : Prop :=
+    | step_atomic e1 σ1 e2 σ2 es t1 t2 :
+        ρ1 = (t1 ++ e1 :: t2, σ1) →
+        ρ2 = (t1 ++ e2 :: t2 ++ es, σ2) →
+        prim_step e1 σ1 κ e2 σ2 es ϕ →
+        step ρ1 κ ρ2 ϕ.
+  #[local] Hint Constructors step : core.
+
+  Inductive nsteps : nat → config Λ → list (observation Λ) → config Λ → list Prop → Prop :=
+    | nsteps_refl ρ :
+       nsteps 0 ρ [] ρ []
+    | nsteps_l n ρ1 ρ2 ρ3 κ κs ϕ ϕs :
+       step ρ1 κ ρ2 ϕ →
+       nsteps n ρ2 κs ρ3 ϕs →
+       nsteps (S n) ρ1 (κ ++ κs) ρ3 (ϕ :: ϕs).
+  #[local] Hint Constructors nsteps : core.
+
+  Lemma of_to_val_flip v e :
+    of_val v = e →
+    to_val e = Some v.
+  Proof.
+    intros <-. rewrite to_of_val //.
+  Qed.
+
+  Lemma not_reducible e σ :
+    ¬ reducible e σ ↔
+    irreducible e σ.
+  Proof.
+    unfold reducible, irreducible. naive_solver.
+  Qed.
+  Lemma reducible_not_val e σ :
+    reducible e σ →
+    to_val e = None.
+  Proof.
+    intros (? & ? & ? & ? & ? & ?); eauto using val_stuck.
+  Qed.
+  Lemma reducible_no_obs_reducible e σ :
+    reducible_no_obs e σ →
+    reducible e σ.
+  Proof.
+    intros (? & ? & ? & ?); eexists; eauto.
+  Qed.
+  Lemma val_irreducible e σ :
+    is_Some (to_val e) →
+    irreducible e σ.
+  Proof.
+    intros [? ?] ? ? ? ? ? ?%val_stuck. destruct (to_val e); done.
+  Qed.
+  #[global] Instance of_val_inj :
+    Inj (=) (=) (@of_val Λ).
+  Proof.
+    intros v v' Hv; apply (inj Some); rewrite -!to_of_val Hv //.
+  Qed.
+  Lemma not_not_stuck e σ :
+    ¬ not_stuck e σ ↔
+    stuck e σ.
+  Proof.
+    rewrite /stuck /not_stuck -not_eq_None_Some -not_reducible.
+    destruct (decide (to_val e = None)); naive_solver.
+  Qed.
+
+  Lemma reducible_fill `{!@LanguageCtx Λ K} e σ :
+    reducible e σ →
+    reducible (K e) σ.
+  Proof.
+    unfold reducible in *. naive_solver eauto using fill_step.
+  Qed.
+  Lemma reducible_fill_inv `{!@LanguageCtx Λ K} e σ :
+    to_val e = None →
+    reducible (K e) σ →
+    reducible e σ.
+  Proof.
+    intros ? (e' & σ' & k & es & ϕ & Hstep); unfold reducible.
+    apply fill_step_inv in Hstep as (e2' & _ & Hstep); naive_solver.
+  Qed.
+  Lemma reducible_no_obs_fill `{!@LanguageCtx Λ K} e σ :
+    reducible_no_obs e σ →
+    reducible_no_obs (K e) σ.
+  Proof.
+    unfold reducible_no_obs in *. naive_solver eauto using fill_step.
+  Qed.
+  Lemma reducible_no_obs_fill_inv `{!@LanguageCtx Λ K} e σ :
+    to_val e = None →
+    reducible_no_obs (K e) σ →
+    reducible_no_obs e σ.
+  Proof.
+    intros ? (e' & σ' & es & ϕ & Hstep); unfold reducible_no_obs.
+    apply fill_step_inv in Hstep as (e2' & _ & Hstep); eauto.
+  Qed.
+  Lemma irreducible_fill `{!@LanguageCtx Λ K} e σ :
+    to_val e = None →
+    irreducible e σ →
+    irreducible (K e) σ.
+  Proof.
+    rewrite -!not_reducible. naive_solver eauto using reducible_fill_inv.
+  Qed.
+  Lemma irreducible_fill_inv `{!@LanguageCtx Λ K} e σ :
+    irreducible (K e) σ →
+    irreducible e σ.
+  Proof.
+    rewrite -!not_reducible. naive_solver eauto using reducible_fill.
+  Qed.
+
+  Lemma not_stuck_fill_inv K `{!@LanguageCtx Λ K} e σ :
+    not_stuck (K e) σ →
+    not_stuck e σ.
+  Proof.
+    rewrite /not_stuck -!not_eq_None_Some. intros [? | ?].
+    - auto using fill_not_val.
+    - destruct (decide (to_val e = None)); eauto using reducible_fill_inv.
+  Qed.
+
+  Lemma stuck_fill `{!@LanguageCtx Λ K} e σ :
+    stuck e σ →
+    stuck (K e) σ.
+  Proof.
+    rewrite -!not_not_stuck. eauto using not_stuck_fill_inv.
+  Qed.
+
+  Lemma step_insert i t2 σ2 e κ e' σ3 es ϕ :
+    t2 !! i = Some e →
+    prim_step e σ2 κ e' σ3 es ϕ →
+    step (t2, σ2) κ (<[i:=e']> t2 ++ es, σ3) ϕ.
+  Proof.
+    intros.
+    edestruct (elem_of_list_split_length t2) as (t21 & t22 & ? & ?).
+    { eauto using elem_of_list_lookup_2. }
+    simplify_eq.
+    econstructor; eauto.
+    rewrite insert_app_r_alt // Nat.sub_diag /= -assoc_L //.
+  Qed.
+
+  Record pure_step e1 e2 := {
+    pure_step_safe σ1 :
+      reducible_no_obs e1 σ1 ;
+    pure_step_det σ1 κ e2' σ2 es ϕ :
+      prim_step e1 σ1 κ e2' σ2 es ϕ →
+        κ = [] ∧
+        σ2 = σ1 ∧
+        e2' = e2 ∧
+        es = [] ;
+  }.
+
+  Notation pure_steps_tp := (
+    Forall2 (rtc pure_step)
+  ).
+
+  Class PureExec (ϕ : Prop) n e1 e2 :=
+    pure_exec :
+      ϕ →
+      relations.nsteps pure_step n e1 e2.
+
+  Lemma pure_step_ctx K `{!@LanguageCtx Λ K} e1 e2 :
+    pure_step e1 e2 →
+    pure_step (K e1) (K e2).
+  Proof.
+    intros [Hred Hstep]. split.
+    - unfold reducible_no_obs in *. naive_solver eauto using fill_step.
+    - intros σ1 κ e2' σ2 es ϕ Hpstep.
+      destruct (fill_step_inv e1 σ1 κ e2' σ2 es ϕ) as (e2'' & -> & ?); [|exact Hpstep|].
+      + destruct (Hred σ1) as (? & ? & ? & ? & ?); eauto using val_stuck.
+      + edestruct (Hstep σ1 κ e2'' σ2 es ϕ) as (? & -> & -> & ->); auto.
+  Qed.
+
+  Lemma pure_step_nsteps_ctx K `{!@LanguageCtx Λ K} n e1 e2 :
+    relations.nsteps pure_step n e1 e2 →
+    relations.nsteps pure_step n (K e1) (K e2).
+  Proof.
+    eauto using nsteps_congruence, pure_step_ctx.
+  Qed.
+
+  Lemma rtc_pure_step_ctx K `{!@LanguageCtx Λ K} e1 e2 :
+    rtc pure_step e1 e2 →
+    rtc pure_step (K e1) (K e2).
+  Proof.
+    eauto using rtc_congruence, pure_step_ctx.
+  Qed.
+
+  Lemma pure_exec_ctx K `{!@LanguageCtx Λ K} ϕ n e1 e2 :
+    PureExec ϕ n e1 e2 →
+    PureExec ϕ n (K e1) (K e2).
+  Proof.
+    rewrite /PureExec; eauto using pure_step_nsteps_ctx.
+  Qed.
+
+  Class IntoVal e v :=
+    into_val : of_val v = e.
+
+  Class AsVal e :=
+    as_val : ∃ v, of_val v = e.
+
+  #[global] Instance as_vals_of_val vs :
+    TCForall AsVal (of_val <$> vs).
+  Proof.
+    apply TCForall_Forall, Forall_fmap, Forall_true => v.
+    rewrite /AsVal /=; eauto.
+  Qed.
+
+  Lemma as_val_is_Some e :
+    (∃ v, of_val v = e) →
+    is_Some (to_val e).
+  Proof.
+    intros [v <-]. rewrite to_of_val. eauto.
+  Qed.
+
+  Lemma prim_step_not_stuck e σ κ e' σ' es ϕ :
+    prim_step e σ κ e' σ' es ϕ →
+    not_stuck e σ.
+  Proof.
+    rewrite /not_stuck /reducible. eauto 10.
+  Qed.
+
+  Lemma rtc_pure_step_val `{!Inhabited (state Λ)} v e :
+    rtc pure_step (of_val v) e →
+    to_val e = Some v.
+  Proof.
+    intros ?; rewrite <- to_of_val.
+    f_equal; symmetry; eapply rtc_nf; first done.
+    intros [e' [Hstep _]].
+    destruct (Hstep inhabitant) as (? & ? & ? & ϕ & Hval%val_stuck).
+    rewrite to_of_val // in Hval.
+  Qed.
+End language.
+
+#[global] Hint Mode PureExec + - - ! - : typeclass_instances.
+
+#[global] Arguments step_atomic {Λ ρ1 κ ρ2 ϕ}.
