theories/iris/program_logic/wp.v
@@ -1,0 +1,570 @@
+From iris.base_logic Require Export
+  lib.fancy_updates.
+
+From zebre Require Import
+  prelude.
+From zebre.iris Require Import
+  diaframe.
+From zebre.iris.program_logic Require Export
+  language.
+From zebre Require Import
+  options.
+
+Class IrisG Λ Σ := {
+  #[global] iris_G_inv_G :: invGS Σ ;
+  state_interp : state Λ → list (observation Λ) → iProp Σ ;
+  fork_post : val Λ → iProp Σ ;
+}.
+#[global] Arguments Build_IrisG {_ _ _} _ _ : assert.
+#[global] Opaque iris_G_inv_G.
+
+Section iris_G.
+  Context `{iris_G : !IrisG Λ Σ}.
+
+  Definition wp_pre (wp : expr Λ -d> coPset -d> (val Λ -d> iPropO Σ) -d> iPropO Σ)
+  : expr Λ -d> coPset -d> (val Λ -d> iPropO Σ) -d> iPropO Σ
+  :=
+    λ e E Φ,
+      match to_val e with
+      | Some v =>
+          |={E}=> Φ v
+      | None =>
+          ∀ σ κ κs,
+          state_interp σ (κ ++ κs) -∗
+            |={E, ∅}=>
+            ⌜reducible e σ⌝ ∗
+              ∀ e' σ' es ϕ,
+              ⌜prim_step e σ κ e' σ' es ϕ⌝ -∗
+              ⌜ϕ⌝ -∗
+              £ 1 -∗
+                |={∅}=> ▷ |={∅, E}=>
+                state_interp σ' κs ∗
+                wp e' E Φ ∗
+                [∗ list] i ↦ e ∈ es,
+                  wp e ⊤ fork_post
+      end%I.
+  #[global] Arguments wp_pre _ e%E E Φ%I : rename.
+
+  #[local] Instance wp_pre_contractive :
+    Contractive wp_pre.
+  Proof.
+    rewrite /wp_pre /= => n wp1 wp2 Hwp e E Φ.
+    repeat (apply Hwp || f_contractive || f_equiv).
+  Qed.
+
+  #[local] Definition wp_def :=
+    fixpoint wp_pre.
+  #[global] Arguments wp_def e%E E Φ%I : rename.
+End iris_G.
+
+#[local] Definition wp_aux : seal (@wp_def).
+  Proof. by eexists. Qed.
+Definition wp :=
+  wp_aux.(unseal).
+#[global] Arguments wp {_ _ _} e%E E Φ%I : rename.
+#[local] Lemma wp_unseal `{iris_G : !IrisG Λ Σ} :
+  wp = @wp_def Λ Σ _.
+Proof.
+  rewrite -wp_aux.(seal_eq) //.
+Qed.
+
+Notation "'WP' e @ E {{ Φ } }" := (
+  wp e%E E Φ
+)(at level 20,
+  e, Φ at level 200,
+  only parsing
+) : bi_scope.
+Notation "'WP' e {{ Φ } }" := (
+  wp e%E ⊤ Φ
+)(at level 20,
+  e, Φ at level 200,
+  only parsing
+) : bi_scope.
+
+Notation "'WP' e @ E {{ v , Q } }" := (
+  wp e%E E (λ v, Q)
+)(at level 20,
+  e, Q at level 200,
+  format "'[hv' 'WP'  e  '/' @  E  '/' {{  '[' v ,  '/' Q  ']' } } ']'"
+) : bi_scope.
+Notation "'WP' e {{ v , Q } }" := (
+  wp e%E ⊤ (λ v, Q)
+)(at level 20,
+  e, Q at level 200,
+  format "'[hv' 'WP'  e  '/' {{  '[' v ,  '/' Q  ']' } } ']'"
+) : bi_scope.
+
+Notation "'{{{' P } } } e @ E {{{ x .. y , 'RET' pat ; Q } } }" :=
+  ( □ ∀ Φ,
+      P -∗
+      ▷ (∀ x, .. (∀ y, Q -∗ Φ pat%V) ..) -∗
+      WP e @ E {{ Φ }}
+  )%I
+( at level 20,
+  x closed binder,
+  y closed binder,
+  format "'[hv' {{{  '[' P  ']' } } }  '/  ' e  '/' @  E  '/' {{{  '[' x  ..  y ,  RET  pat ;  '/' Q  ']' } } } ']'"
+) : bi_scope.
+Notation "'{{{' P } } } e {{{ x .. y , 'RET' pat ; Q } } }" :=
+  ( □ ∀ Φ,
+      P -∗
+      ▷ (∀ x, .. (∀ y, Q -∗ Φ pat%V) ..) -∗
+      WP e {{ Φ }}
+  )%I
+( at level 20,
+  x closed binder,
+  y closed binder,
+  format "'[hv' {{{  '[' P  ']' } } }  '/  ' e  '/' {{{  '[' x  ..  y ,  RET  pat ;  '/' Q  ']' } } } ']'"
+) : bi_scope.
+
+Notation "'{{{' P } } } e @ E {{{ 'RET' pat ; Q } } }" :=
+  ( □ ∀ Φ,
+      P -∗
+      ▷ (Q -∗ Φ pat%V) -∗
+      WP e @ E {{ Φ }}
+  )%I
+( at level 20,
+  format "'[hv' {{{  '[' P  ']' } } }  '/  ' e  '/' @  E  '/' {{{  '[' RET  pat ;  '/' Q  ']' } } } ']'"
+) : bi_scope.
+Notation "'{{{' P } } } e {{{ 'RET' pat ; Q } } }" :=
+  ( □ ∀ Φ,
+      P -∗
+      ▷ (Q -∗ Φ pat%V) -∗
+      WP e {{ Φ }}
+  )%I
+( at level 20,
+  format "'[hv' {{{  '[' P  ']' } } }  '/  ' e  '/' {{{  '[' RET  pat ;  '/' Q  ']' } } } ']'"
+) : bi_scope.
+
+Notation "'{{{' P } } } e @ E {{{ x .. y , 'RET' pat ; Q } } }" := (
+  ∀ Φ,
+  P -∗
+  ▷ (∀ x, .. (∀ y, Q -∗ Φ pat%V) ..) -∗
+  WP e @ E {{ Φ }}
+) : stdpp_scope.
+Notation "'{{{' P } } } e {{{ x .. y , 'RET' pat ; Q } } }" := (
+  ∀ Φ,
+  P -∗
+  ▷ (∀ x, .. (∀ y, Q -∗ Φ pat%V) ..) -∗
+  WP e {{ Φ }}
+) : stdpp_scope.
+Notation "'{{{' P } } } e @ E {{{ 'RET' pat ; Q } } }" := (
+  ∀ Φ,
+  P -∗
+  ▷ (Q -∗ Φ pat%V) -∗
+  WP e @ E {{ Φ }}
+) : stdpp_scope.
+Notation "'{{{' P } } } e {{{ 'RET' pat ; Q } } }" := (
+  ∀ Φ,
+  P -∗
+  ▷ (Q -∗ Φ pat%V) -∗
+  WP e {{ Φ }}
+) : stdpp_scope.
+
+Section iris_G.
+  Context `{iris_G : !IrisG Λ Σ}.
+
+  Implicit Types e : expr Λ.
+  Implicit Types v : val Λ.
+  Implicit Types P R : iProp Σ.
+  Implicit Types Φ : val Λ → iProp Σ.
+
+  Lemma wp_unfold e E Φ :
+    WP e @ E {{ Φ }} ⊣⊢
+    wp_pre wp e E Φ.
+  Proof.
+    rewrite wp_unseal. apply (fixpoint_unfold wp_pre).
+  Qed.
+
+  #[global] Instance wp_ne n e E :
+    Proper (pointwise_relation _ (≡{n}≡) ==> (≡{n}≡)) (wp e E).
+  Proof.
+    move: e. induction (lt_wf n) as [n _ IH] => e Φ1 Φ2 HΦ.
+    rewrite !wp_unfold /wp_pre /=.
+    do 26 (f_contractive || f_equiv).
+    apply IH; first done.
+    f_equiv.
+    eapply dist_le; [apply HΦ | lia].
+  Qed.
+  #[global] Instance wp_proper e E :
+    Proper (pointwise_relation _ (≡) ==> (≡)) (wp e E).
+  Proof.
+    intros Φ1 Φ2 HΦ.
+    apply equiv_dist => n. apply wp_ne => v. apply equiv_dist. done.
+  Qed.
+  #[global] Instance wp_contractive n e E :
+    TCEq (to_val e) None →
+    Proper (pointwise_relation _ (dist_later n) ==> (≡{n}≡)) (wp e E).
+  Proof.
+    intros He Φ1 Φ2 HΦ.
+    rewrite !wp_unfold /wp_pre He /=.
+    repeat (f_contractive || f_equiv).
+  Qed.
+
+  Lemma wp_value_fupd' v E Φ :
+    WP of_val v @ E {{ Φ }} ⊣⊢
+    |={E}=> Φ v.
+  Proof.
+    rewrite wp_unfold /wp_pre to_of_val //.
+  Qed.
+
+  Lemma wp_strong_mono e E1 Φ1 E2 Φ2 :
+    E1 ⊆ E2 →
+    WP e @ E1 {{ Φ1 }} -∗
+    (∀ v, Φ1 v ={E2}=∗ Φ2 v) -∗
+    WP e @ E2 {{ Φ2 }}.
+  Proof.
+    iIntros "%HE H HΦ".
+    iLöb as "HLöb" forall (e).
+    rewrite !wp_unfold /wp_pre /=.
+    destruct (to_val e) as [v |] eqn:He.
+    - iApply ("HΦ" with "[> H]").
+      iSteps.
+    - iIntros "%σ1 %κ %κs Hσ".
+      iMod (fupd_mask_subseteq E1) as "Hclose"; first done.
+      iMod ("H" with "Hσ") as "(%Hreducible & H)".
+      iModIntro. iStep. iIntros "%e2 %σ2 %es %ϕ %Hstep %Hϕ H£".
+      iMod ("H" with "[//] [//] H£") as "H".
+      do 2 iModIntro.
+      iMod "H" as "($ & H & Hes)".
+      iMod "Hclose" as "_".
+      iSplitR "Hes"; iSteps.
+  Qed.
+
+  Lemma fupd_wp e E Φ :
+    (|={E}=> WP e @ E {{ Φ }}) ⊢
+    WP e @ E {{ Φ }}.
+  Proof.
+    iIntros "H".
+    rewrite wp_unfold /wp_pre.
+    destruct (to_val e) as [v |] eqn:He; first iSteps.
+    iIntros "%σ1 %κ %κs Hσ".
+    iMod "H".
+    iApply ("H" with "Hσ").
+  Qed.
+  Lemma wp_fupd e E Φ :
+    WP e @ E {{ v, |={E}=> Φ v }} ⊢
+    WP e @ E {{ Φ }}.
+  Proof.
+    iIntros "H".
+    iApply (wp_strong_mono with "H"); first done.
+    iSteps.
+  Qed.
+
+  Lemma wp_atomic e `{!Atomic e} E1 E2 Φ :
+    (|={E1, E2}=> WP e @ E2 {{ v, |={E2, E1}=> Φ v }}) ⊢
+    WP e @ E1 {{ Φ }}.
+  Proof.
+    iIntros "H".
+    rewrite !wp_unfold /wp_pre.
+    destruct (to_val e) as [v |] eqn:He; first iSteps.
+    iIntros "%σ1 %κ1 %κs Hσ".
+    iMod "H".
+    iMod ("H" $! σ1 with "Hσ") as "($ & H)".
+    iModIntro. iIntros "%e2 %σ2 %es1 %ϕ1 %Hstep1 %Hϕ1 H£".
+    iMod ("H" with "[//] [//] H£") as "H".
+    do 2 iModIntro.
+    iMod "H" as "(Hσ & H & Hes)".
+    rewrite !wp_unfold /wp_pre.
+    destruct (to_val e2) as [v2 |] eqn:He2.
+    - iDestruct "H" as ">>$".
+      iSteps.
+    - iMod ("H" $! _ [] with "Hσ") as "(%Hreducible2 & _)".
+      destruct Hreducible2 as (κ2 & e3 & σ3 & es2 & ϕ2 & Hstep2).
+      edestruct atomic; [done | congruence].
+  Qed.
+
+  Lemma wp_step_fupd e E1 E2 P Φ :
+    TCEq (to_val e) None →
+    E2 ⊆ E1 →
+    (|={E1}[E2]▷=> P) -∗
+    WP e @ E2 {{ v, P ={E1}=∗ Φ v }} -∗
+    WP e @ E1 {{ Φ }}.
+  Proof.
+    rewrite !wp_unfold /wp_pre /=.
+    iIntros (-> HE) "HP H %σ1 %κ1 %κs Hσ".
+    iMod "HP".
+    iMod ("H" with "Hσ") as "($ & H)".
+    iIntros "!> %e2 %σ2 %es1 %ϕ1 %Hstep %Hϕ H£".
+    iMod ("H" with "[//] [//] H£") as "H".
+    do 2 iModIntro.
+    iMod "H" as "($ & H & $)".
+    iMod "HP".
+    iApply (wp_strong_mono with "H"); first done.
+    iSteps.
+  Qed.
+
+  Lemma wp_bind K `{!LanguageCtx K} e E Φ :
+    WP e @ E {{ v, WP K (of_val v) @ E {{ Φ }} }} ⊢
+    WP K e @ E {{ Φ }}.
+  Proof.
+    iIntros "H".
+    iLöb as "IH" forall (e).
+    rewrite wp_unfold /wp_pre.
+    destruct (to_val e) as [v |] eqn:He.
+    - apply of_to_val in He as <-.
+      iApply (fupd_wp with "H").
+    - rewrite wp_unfold /wp_pre fill_not_val //.
+      iIntros "%σ1 %κ1 %κs Hσ".
+      iMod ("H" with "Hσ") as "(%Hreducible1 & H)".
+      iModIntro; iSplit; first eauto using reducible_fill.
+      iIntros "%e2 %σ2 %es1 %ϕ1 %Hstep1 %Hϕ1 H£".
+      destruct (fill_step_inv e σ1 κ1 e2 σ2 es1 ϕ1) as (e2' & -> & Hstep1'); [done.. |].
+      iMod ("H" with "[//] [//] H£") as "H".
+      iModIntro. iSteps.
+  Qed.
+
+  Lemma wp_bind_inv K `{!LanguageCtx K} e E Φ :
+    WP K e @ E {{ Φ }} ⊢
+    WP e @ E {{ v, WP K (of_val v) @ E {{ Φ }} }}.
+  Proof.
+    iIntros "H".
+    iLöb as "IH" forall (e).
+    rewrite !wp_unfold /wp_pre /=.
+    destruct (to_val e) as [v |] eqn:He.
+    - apply of_to_val in He as <-.
+      rewrite !wp_unfold /wp_pre //.
+    - rewrite fill_not_val //.
+      iIntros "%σ1 %κ1 %κs Hσ".
+      iMod ("H" with "Hσ") as "(%Hreducible & H)".
+      iModIntro; iSplit; first eauto using reducible_fill_inv.
+      iIntros "%e2 %σ2 %es1 %ϕ1 %Hstep1 %Hϕ1 H£".
+      iMod ("H" with "[] [//] H£") as "H"; first eauto using fill_step.
+      iModIntro. iSteps.
+  Qed.
+
+  Lemma wp_mono e E Φ1 Φ2 :
+    (∀ v, Φ1 v ⊢ Φ2 v) →
+    WP e @ E {{ Φ1 }} ⊢
+    WP e @ E {{ Φ2 }}.
+  Proof.
+    iIntros "%HΦ H".
+    iApply (wp_strong_mono with "H"); first done. iIntros "%v HΦ".
+    iApply (HΦ with "HΦ").
+  Qed.
+  Lemma wp_mask_mono e E1 E2 Φ :
+    E1 ⊆ E2 →
+    WP e @ E1 {{ Φ }} ⊢
+    WP e @ E2 {{ Φ }}.
+  Proof.
+    iIntros "%HE H".
+    iApply (wp_strong_mono with "H"); first done.
+    iSteps.
+  Qed.
+  #[global] Instance wp_mono' e E :
+    Proper (pointwise_relation _ (⊢) ==> (⊢)) (wp e E).
+  Proof.
+    intros Φ1 Φ2 HΦ.
+    apply wp_mono. done.
+  Qed.
+  #[global] Instance wp_flip_mono' e E :
+    Proper (pointwise_relation _ (flip (⊢)) ==> (flip (⊢))) (wp e E).
+  Proof.
+    intros Φ1 Φ2 HΦ.
+    apply wp_mono. done.
+  Qed.
+
+  Lemma wp_value_fupd e v E Φ :
+    IntoVal e v →
+    WP e @ E {{ Φ }} ⊣⊢
+    |={E}=> Φ v.
+  Proof.
+    rewrite -wp_value_fupd' => <- //.
+  Qed.
+  Lemma wp_value' v E Φ :
+    Φ v ⊢
+    WP (of_val v) @ E {{ Φ }}.
+  Proof.
+    rewrite wp_value_fupd'. auto.
+  Qed.
+  Lemma wp_value e v E Φ :
+    IntoVal e v →
+    Φ v ⊢
+    WP e @ E {{ Φ }}.
+  Proof.
+    rewrite wp_value' => <- //.
+  Qed.
+
+  Lemma wp_frame_l e E Φ R :
+    R ∗ WP e @ E {{ Φ }} ⊢
+    WP e @ E {{ v, R ∗ Φ v }}.
+  Proof.
+    iIntros "(HR & H)".
+    iApply (wp_strong_mono with "H"); first done.
+    iSteps.
+  Qed.
+  Lemma wp_frame_r e E Φ R :
+    WP e @ E {{ Φ }} ∗ R ⊢
+    WP e @ E {{ v, Φ v ∗ R }}.
+  Proof.
+    iIntros "(H & HR)".
+    iApply (wp_strong_mono with "H"); first done.
+    iSteps.
+  Qed.
+
+  Lemma wp_wand e E Φ1 Φ2 :
+    WP e @ E {{ Φ1 }} -∗
+    (∀ v, Φ1 v -∗ Φ2 v) -∗
+    WP e @ E {{ Φ2 }}.
+  Proof.
+    iIntros "H HΦ".
+    iApply (wp_strong_mono with "H"); first done.
+    iSteps.
+  Qed.
+  Lemma wp_wand_l e E Φ1 Φ2 :
+    (∀ v, Φ1 v -∗ Φ2 v) ∗ WP e @ E {{ Φ1 }} ⊢
+    WP e @ E {{ Φ2 }}.
+  Proof.
+    iIntros "(HΦ & H)".
+    iApply (wp_wand with "H HΦ").
+  Qed.
+  Lemma wp_wand_r e E Φ1 Φ2 :
+    WP e @ E {{ Φ1 }} ∗ (∀ v, Φ1 v -∗ Φ2 v) ⊢
+    WP e @ E {{ Φ2 }}.
+  Proof.
+    iIntros "(H & HΦ)".
+    iApply (wp_wand with "H HΦ").
+  Qed.
+  Lemma wp_frame_wand e E Φ R :
+    R -∗
+    WP e @ E {{ v, R -∗ Φ v }} -∗
+    WP e @ E {{ Φ }}.
+  Proof.
+    iIntros "HR H".
+    iApply (wp_wand with "H").
+    iSteps.
+  Qed.
+
+  #[global] Instance frame_wp p e E R Φ1 Φ2 :
+    (∀ v, Frame p R (Φ1 v) (Φ2 v)) →
+    Frame
+      p
+      R
+      (WP e @ E {{ Φ1 }})
+      (WP e @ E {{ Φ2 }})
+  | 2.
+  Proof.
+    rewrite /Frame wp_frame_l => HR.
+    apply wp_mono, HR.
+  Qed.
+
+  #[global] Instance is_except_0_wp e E Φ :
+    IsExcept0 (WP e @ E {{ Φ }}).
+  Proof.
+    rewrite /IsExcept0 -{2}fupd_wp -except_0_fupd -fupd_intro //.
+  Qed.
+
+  #[global] Instance elim_modal_bupd_wp p e E P Φ :
+    ElimModal
+      True
+      p
+      false
+      (|==> P)
+      P
+      (WP e @ E {{ Φ }})
+      (WP e @ E {{ Φ }}).
+  Proof.
+    rewrite /ElimModal bi.intuitionistically_if_elim (bupd_fupd E) fupd_frame_r bi.wand_elim_r fupd_wp //.
+  Qed.
+
+  #[global] Instance elim_modal_fupd_wp p e E P Φ :
+    ElimModal
+      True
+      p
+      false
+      (|={E}=> P)
+      P
+      (WP e @ E {{ Φ }})
+      (WP e @ E {{ Φ }}).
+  Proof.
+    rewrite /ElimModal bi.intuitionistically_if_elim fupd_frame_r bi.wand_elim_r fupd_wp //.
+  Qed.
+  #[global] Instance elim_modal_fupd_wp_wrong_mask p e E1 E2 P Φ :
+    ElimModal
+      (pm_error "Goal and eliminated modality must have the same mask.
+Use [iApply fupd_wp; iMod (fupd_mask_subseteq E2)] to adjust the mask of your goal to [E2]")
+      p
+      false
+      (|={E2}=> P)
+      False
+      (WP e @ E1 {{ Φ }})
+      False
+  | 100.
+  Proof.
+    intros [].
+  Qed.
+
+  #[global] Instance elim_modal_fupd_wp_atomic p e E1 E2 P Φ :
+    ElimModal
+      (Atomic e)
+      p
+      false
+      (|={E1,E2}=> P)
+      P
+      (WP e @ E1 {{ Φ }})
+      (WP e @ E2 {{ v, |={E2,E1}=> Φ v }})%I
+  | 100.
+  Proof.
+    intros He.
+    rewrite bi.intuitionistically_if_elim fupd_frame_r bi.wand_elim_r wp_atomic //.
+  Qed.
+  #[global] Instance elim_modal_fupd_wp_atomic_wrong_mask p e E1 E2 E2' P Φ :
+    ElimModal
+      (pm_error "Goal and eliminated modality must have the same mask.
+Use [iMod (fupd_mask_subseteq E2)] to adjust the mask of your goal to [E2]")
+      p
+      false
+      (|={E2,E2'}=> P)
+      False
+      (WP e @ E1 {{ Φ }})
+      False
+  | 200.
+  Proof.
+    intros [].
+  Qed.
+
+  #[global] Instance add_modal_fupd_wp e E P Φ :
+    AddModal
+      (|={E}=> P)
+      P
+      (WP e @ E {{ Φ }}).
+  Proof.
+    rewrite /AddModal fupd_frame_r bi.wand_elim_r fupd_wp //.
+  Qed.
+
+  #[global] Instance elim_acc_wp_atomic {X} e E1 E2 α β γ Φ :
+    ElimAcc (X := X)
+      (Atomic e)
+      (fupd E1 E2)
+      (fupd E2 E1)
+      α
+      β
+      γ
+      (WP e @ E1 {{ Φ }})
+      (λ x, WP e @ E2 {{ v, |={E2}=> β x ∗ (γ x -∗? Φ v) }})%I
+  | 100.
+  Proof.
+    iIntros "%He Hinner >Hacc".
+    iDestruct "Hacc" as "(%x & Hα & Hclose)".
+    iApply (wp_wand with "(Hinner Hα)"). iIntros "%v >(Hβ & HΦ)".
+    iApply ("HΦ" with "(Hclose Hβ)").
+  Qed.
+
+  #[global] Instance elim_acc_wp_nonatomic {X} e E α β γ Φ :
+    ElimAcc (X := X)
+      True
+      (fupd E E)
+      (fupd E E)
+      α
+      β
+      γ
+      (WP e @ E {{ Φ }})
+      (λ x, WP e @ E {{ v, |={E}=> β x ∗ (γ x -∗? Φ v) }})%I.
+  Proof.
+    iIntros (_) "Hinner >Hacc".
+    iDestruct "Hacc" as "(%x & Hα & Hclose)".
+    iApply wp_fupd.
+    iApply (wp_wand with "(Hinner Hα)"). iIntros "%v >(Hβ & HΦ)".
+    iApply ("HΦ" with "(Hclose Hβ)").
+  Qed.
+End iris_G.
