theories/iris/program_logic/wp_lifting.v
@@ -1,0 +1,221 @@
+From zebre Require Import
+  prelude.
+From zebre.iris Require Import
+  diaframe.
+From zebre.iris.program_logic Require Import
+  ectx_language.
+From zebre.iris.program_logic Require Export
+  wp.
+From zebre Require Import
+  options.
+
+Section language.
+  Context `{iris_G : !IrisG Λ Σ}.
+
+  Implicit Types e : expr Λ.
+  Implicit Types Φ : val Λ → iProp Σ.
+
+  Lemma wp_lift_step e E Φ :
+    to_val e = None →
+    ( ∀ σ κ κs,
+      state_interp σ (κ ++ κs) -∗
+        |={E, ∅}=>
+        ⌜reducible e σ⌝ ∗
+          ∀ e' σ' es ϕ,
+          ⌜prim_step e σ κ e' σ' es ϕ⌝ -∗
+          ⌜ϕ⌝ -∗
+          £ 1 -∗
+            |={∅}=> ▷ |={∅, E}=>
+            state_interp σ' κs ∗
+            wp e' E Φ ∗
+            [∗ list] i ↦ e ∈ es,
+              wp e ⊤ fork_post
+    ) ⊢
+    WP e @ E {{ Φ }}.
+  Proof.
+    rewrite wp_unfold /wp_pre => -> //.
+  Qed.
+
+  Lemma wp_lift_atomic_step e E1 E2 Φ :
+    to_val e = None →
+    ( ∀ σ κ κs,
+      state_interp σ (κ ++ κs) -∗
+        |={E1}=>
+        ⌜reducible e σ⌝ ∗
+          ∀ e' σ' es ϕ,
+          ⌜prim_step e σ κ e' σ' es ϕ⌝ -∗
+          ⌜ϕ⌝ -∗
+          £ 1 -∗
+            |={E1}[E2]▷=>
+            state_interp σ' κs ∗
+            from_option Φ False (to_val e') ∗
+            [∗ list] e ∈ es,
+              WP e @ ⊤ {{ fork_post }}
+    ) ⊢
+    WP e @ E1 {{ Φ }}.
+  Proof.
+    iIntros "%He H".
+    iApply wp_lift_step; first done. iIntros "%σ %κ %κs Hσ".
+    iMod ("H" $! σ with "Hσ") as "($ & H)".
+    iApply fupd_mask_intro; first set_solver. iIntros "Hclose %e' %σ' %es %ϕ %Hstep %Hϕ H£".
+    iMod "Hclose" as "_".
+    iMod ("H" with "[//] [//] H£") as "H".
+    iApply fupd_mask_intro; first set_solver. iIntros "Hclose !>".
+    iMod "Hclose" as "_".
+    iMod "H" as "($ & HΦ & $)".
+    destruct (to_val e') eqn:He'; last by iExFalso.
+    iApply (wp_value with "HΦ").
+    apply of_to_val. done.
+  Qed.
+
+  Lemma wp_lift_pure_step_no_fork `{!Inhabited (state Λ)} e E1 E2 Φ :
+    ( ∀ σ,
+      reducible e σ
+    ) →
+    ( ∀ σ κ e' σ' es ϕ,
+      prim_step e σ κ e' σ' es ϕ →
+        κ = [] ∧
+        σ' = σ ∧
+        es = []
+    ) →
+    ( |={E1}[E2]▷=>
+      ∀ σ e' κ es ϕ,
+      ⌜prim_step e σ κ e' σ es ϕ⌝ -∗
+      £ 1 -∗
+      WP e' @ E1 {{ Φ }}
+    ) ⊢
+    WP e @ E1 {{ Φ }}.
+  Proof.
+    iIntros "%Hsafe %Hpure H".
+    iApply wp_lift_step.
+    { specialize (Hsafe inhabitant). eauto using reducible_not_val. }
+    iIntros (σ κ κs ) "Hσ".
+    iMod "H".
+    iApply fupd_mask_intro; first set_solver. iIntros "Hclose".
+    iSplit; first iSteps. iIntros "%e' %σ' %es %ϕ %Hstep %Hϕ H£ !> !>".
+    destruct (Hpure σ κ e' σ' es ϕ) as (-> & <- & ->); first done.
+    iSteps.
+  Qed.
+
+  Lemma wp_lift_pure_det_step_no_fork `{!Inhabited (state Λ)} e1 e2 E1 E2 Φ :
+    ( ∀ σ1,
+      reducible e1 σ1
+    ) →
+    ( ∀ σ1 κ e2' σ2 es ϕ,
+      prim_step e1 σ1 κ e2' σ2 es ϕ →
+        κ = [] ∧
+        σ2 = σ1 ∧
+        e2' = e2 ∧
+        es = []
+    ) →
+    ( |={E1}[E2]▷=>
+      £ 1 -∗
+      WP e2 @ E1 {{ Φ }}
+    ) ⊢
+    WP e1 @ E1 {{ Φ }}.
+  Proof.
+    iIntros "%Hsafe %Hpure H".
+    iApply (wp_lift_pure_step_no_fork); [done | naive_solver |].
+    iApply (step_fupd_wand with "H"). iIntros "H %σ1 %e2' %κ %es %ϕ %Hstep H£".
+    apply Hpure in Hstep as (-> & _ & -> & ->).
+    iSteps.
+  Qed.
+
+  Lemma wp_pure_step `{!Inhabited (state Λ)} ψ n e1 e2 E1 E2 Φ :
+    PureExec ψ n e1 e2 →
+    ψ →
+    ( |={E1}[E2]▷=>^n
+      £ n -∗
+      WP e2 @ E1 {{ Φ }}
+    ) ⊢
+    WP e1 @ E1 {{ Φ }}.
+  Proof.
+    iIntros "%Hexec %Hψ H".
+    specialize (Hexec Hψ).
+    iInduction Hexec as [e | n e1 e2 e3 (Hsafe & Hpure)] "IH" => /=.
+    - iMod lc_zero as "H£".
+      iSteps.
+    - iApply wp_lift_pure_det_step_no_fork.
+      + eauto using reducible_no_obs_reducible.
+      + done.
+      + iApply (step_fupd_wand with "H"). iIntros "H H£".
+        iApply "IH".
+        iApply (step_fupdN_wand with "H").
+        rewrite (lc_succ n). iSteps.
+  Qed.
+  Lemma wp_pure_step_later `{!Inhabited (state Λ)} ψ n e1 e2 E Φ :
+    PureExec ψ n e1 e2 →
+    ψ →
+    ▷^n (
+      £ n -∗
+      WP e2 @ E {{ Φ }}
+    ) ⊢
+    WP e1 @ E {{ Φ }}.
+  Proof.
+    intros Hexec Hψ.
+    rewrite -wp_pure_step // {Hexec}.
+    enough (∀ P, ▷^n P ⊢ |={E}▷=>^n P) as H by apply H.
+    intros P. induction n as [| n IH]; rewrite //= -step_fupd_intro // IH //.
+  Qed.
+End language.
+
+Section ectx_language.
+  Context {Λ : ectx_language} `{iris_G : !IrisG Λ Σ}.
+
+  Implicit Types e : expr Λ.
+  Implicit Types Φ : val Λ → iProp Σ.
+
+  #[local] Hint Resolve
+    base_prim_reducible
+    base_reducible_prim_step
+  : core.
+
+  Lemma wp_lift_atomic_base_step e E1 E2 Φ :
+    to_val e = None →
+    ( ∀ σ κ κs,
+      state_interp σ (κ ++ κs) -∗
+        |={E1}=>
+        ⌜base_reducible e σ⌝ ∗
+        ∀ e' σ' es ϕ,
+        ⌜base_step e σ κ e' σ' es ϕ⌝ -∗
+        £ 1 -∗
+          |={E1}[E2]▷=>
+          state_interp σ' κs ∗
+          from_option Φ False (to_val e') ∗
+          [∗ list] e ∈ es,
+            WP e @ ⊤ {{ fork_post }}
+    ) ⊢
+    WP e @ E1 {{ Φ }}.
+  Proof.
+    iIntros "%He H".
+    iApply wp_lift_atomic_step; first done. iIntros "%σ %κ %κs Hσ".
+    iMod ("H" with "Hσ") as "(%Hreducible & H)".
+    iModIntro. iSplit; first iSteps. iIntros "%e' %σ' %es %ϕ %Hstep Hϕ".
+    iApply "H".
+    iSteps.
+  Qed.
+
+  Lemma wp_lift_atomic_base_step_no_fork e E1 E2 Φ :
+    to_val e = None →
+    ( ∀ σ κ κs,
+      state_interp σ (κ ++ κs) -∗
+        |={E1}=>
+        ⌜base_reducible e σ⌝ ∗
+          ∀ e' σ' es ϕ,
+          ⌜base_step e σ κ e' σ' es ϕ⌝ -∗
+          £ 1 -∗
+            |={E1}[E2]▷=>
+            ⌜es = []⌝ ∗
+            state_interp σ' κs ∗
+            from_option Φ False (to_val e')
+    ) ⊢
+    WP e @ E1 {{ Φ }}.
+  Proof.
+    iIntros "%He H".
+    iApply wp_lift_atomic_base_step; first done. iIntros "%σ %κ %κs Hσ".
+    iMod ("H" with "Hσ") as "($ & H)".
+    iModIntro. iIntros "%e' %σ' %es %ϕ %Hstep H£".
+    iMod ("H" with "[//] H£") as "H".
+    iModIntro. iSteps.
+  Qed.
+End ectx_language.
