theories/language/adequacy.v
@@ -1,8 +1,7 @@
-From iris.program_logic Require Export
-  adequacy.
-
 From zebre Require Import
   prelude.
+From zebre.iris.program_logic Require Export
+  adequacy.
 From zebre.iris Require Import
   diaframe.
 From zebre.language Require Export
@@ -20,11 +19,11 @@ Definition zebre_adequacy Σ `{zebre_Gpre : !ZebreGpre Σ} e σ ϕ :
   ( ∀ `{zebre_G : !ZebreG Σ},
     ⊢ WP e @ ⊤ {{ v, ⌜ϕ v⌝ }}
   ) →
-  adequate NotStuck e σ (λ v σ, ϕ v).
+  adequate e σ.
 Proof.
   intros Hwp.
   apply: wp_adequacy => Hinv_G κs.
   iMod zebre_init as "(%zebre_G & Hσ)".
-  iExists zebre_state_interp, (λ _, True%I). iFrame.
+  iExists zebre_state_interp, (λ _, True%I), _. iFrame.
   iApply (Hwp (Build_ZebreG Σ)).
 Qed.
