theories/language/language.v
@@ -1,10 +1,9 @@
-From iris.program_logic Require Export
+From zebre Require Import
+  prelude.
+From zebre.iris.program_logic Require Export
   language
   ectx_language
   ectxi_language.
-
-From zebre Require Import
-  prelude.
 From zebre.language Require Export
   semantics.
 From zebre Require Import
@@ -32,7 +31,7 @@ Proof.
 Qed.
 
 Canonical zebre_ectxi_lang :=
-  EctxiLanguage zebre_mixin.
+  Build_ectxi_language zebre_mixin.
 Canonical zebre_ectx_lang :=
   EctxLanguageOfEctxi zebre_ectxi_lang.
 Canonical zebre :=
@@ -51,19 +50,19 @@ Proof.
   { destruct k; simpl; apply fill_not_val; done. }
   simplify_eq.
 Qed.
-Lemma prim_step_to_val_is_base_step e σ1 κ v σ2 es :
-  prim_step e σ1 κ (Val v) σ2 es →
-  base_step e σ1 κ (Val v) σ2 es.
+Lemma prim_step_to_val_is_base_step e σ1 κ v σ2 es ϕ :
+  prim_step e σ1 κ (Val v) σ2 es ϕ →
+  base_step e σ1 κ (Val v) σ2 es ϕ.
 Proof.
   intro H. destruct H as [K e1 e2 H1 H2].
   assert (to_val (fill K e2) = Some v) as H3; first rewrite -H2 //.
   apply to_val_fill_some in H3 as [-> ->]. subst e. done.
 Qed.
-Lemma base_step_to_val e1 σ1 κ e2 σ2 es σ1' κ' e2' σ2' es' :
-  base_step e1 σ1 κ e2 σ2 es →
-  base_step e1 σ1' κ' e2' σ2' es' →
-  is_Some (to_val e2) →
-  is_Some (to_val e2').
+Lemma base_step_to_val e σ1 κ1 e1 σ1' es1 ϕ1 σ2 κ2 e2 σ2' es2 ϕ2 :
+  base_step e σ1 κ1 e1 σ1' es1 ϕ1 →
+  base_step e σ2 κ2 e2 σ2' es2 ϕ2 →
+  is_Some (to_val e1) →
+  is_Some (to_val e2).
 Proof.
   destruct 1; inversion 1; naive_solver.
 Qed.
@@ -72,7 +71,7 @@ Lemma irreducible_resolve e v1 v2 σ :
   irreducible e σ →
   irreducible (Resolve e (Val v1) (Val v2)) σ.
 Proof.
-  intros H κ ? σ' es [K' e1' e2' Hfill -> step]. simpl in *.
+  intros H κ ? σ' es ϕ [K' e1' e2' Hfill -> step]. simpl in *.
   induction K' as [| K K' _] using rev_ind; simpl in Hfill.
   - subst e1'. inversion step. eapply H. apply base_prim_step. done.
   - rewrite fill_app /= in Hfill.
